Consolidate and generalize data structure proofs.
Signed-off-by: Emina Torlak <torlaket@amazon.com>

cedar-lean/Cedar/Data/Map.lean
@@ -22,7 +22,7 @@ list of key-value. Functions maps assume but don't require that their inputs are
 well-formed (sorted and duplicate-free). Separate theorems show that these
 functions produce well-formed outputs when given well-formed inputs.
 
-Use Map.make to construct well-formed maps from lists of key-value pairs.
+Use `Map.make` to construct well-formed maps from lists of key-value pairs.
 -/
 
 namespace Cedar.Data
@@ -33,23 +33,20 @@ deriving Repr, DecidableEq, Repr, Inhabited
 
 namespace Map
 
-def kvs {α : Type u} {β : Type v} : Map α β → List (Prod α β)
-| .mk kvs => kvs
-
-
-open Except
+abbrev kvs  {α : Type u} {β : Type v} (m : Map α β) := m.1
 
 ----- Definitions -----
 
--- produces an ordered and duplicate free list provided the given map is well formed
-def toList {α : Type u} {β : Type v} (m : Map α β) : List (Prod α β) := m.kvs
-
-/- Creates a well-formed map from the given list of pairs. -/
+/-- Creates a well-formed map from the given list of pairs. -/
 def make {α β} [LT α] [DecidableLT α] (kvs : List (α × β)) : Map α β :=
   Map.mk (kvs.canonicalize Prod.fst)
 
 /-- Empty map -/
 def empty {α β} : Map α β := .mk []
+
+/-- Returns an ordered and duplicate free list provided the given map is well-formed. -/
+def toList {α : Type u} {β : Type v} (m : Map α β) : List (Prod α β) := m.kvs
+
 
 /-- Returns the keys of `m` as a set. -/
 def keys {α β} (m : Map α β) : Set α :=
@@ -57,7 +54,7 @@ def keys {α β} (m : Map α β) : Set α :=
 
 /-- Returns the binding for `k` in `m`, if any. -/
 def find? {α β} [BEq α] (m : Map α β) (k : α) : Option β :=
-  match m.kvs.find? (fun ⟨k', _⟩ => k' == k) with
+  match m.kvs.find? (λ ⟨k', _⟩ => k' == k) with
   | some (_, v) => some v
   | _           => none
 
@@ -68,8 +65,8 @@ def contains {α β} [BEq α] (m : Map α β) (k : α) : Bool :=
 /-- Returns the binding for `k` in `m` or `err` if none is found. -/
 def findOrErr {α β ε} [BEq α] (m : Map α β) (k : α) (err: ε) : Except ε β :=
   match m.find? k with
-  | some v => ok v
-  | _      => error err
+  | some v => .ok v
+  | _      => .error err
 
 /-- Returns the binding for `k` in `m`, or panics if none is found. -/
 def find! {α β} [Repr α] [BEq α] [Inhabited β] (m : Map α β) (k : α) : β :=
@@ -79,42 +76,28 @@ def find! {α β} [Repr α] [BEq α] [Inhabited β] (m : Map α β) (k : α) : �
 
 /-- Filters `m` using `f`. -/
 def filter {α β} (f : α → β → Bool) (m : Map α β) : Map α β :=
-  Map.mk (m.kvs.filter (fun ⟨k, v⟩ => f k v))
+  Map.mk (m.kvs.filter (λ ⟨k, v⟩ => f k v))
 
 def size {α β} (m : Map α β) : Nat :=
   m.kvs.length
 
 def mapOnValues {α β γ} [LT α] [DecidableLT α] (f : β → γ) (m : Map α β) : Map α γ :=
-  Map.mk (m.kvs.map (λ (k,v) => (k, f v)))
+  Map.mk (m.kvs.map (λ (k, v) => (k, f v)))
 
 def mapOnKeys {α β γ} [LT γ] [DecidableLT γ] (f : α → γ) (m : Map α β) : Map γ β :=
-  Map.make (m.kvs.map (λ (k,v) => (f k, v)))
+  Map.make (m.kvs.map (λ (k, v) => (f k, v)))
 
------ Props and Theorems -----
+----- Instances -----
 
 instance [LT (Prod α β)] : LT (Map α β) where
-lt a b := a.kvs < b.kvs
+  lt a b := a.kvs < b.kvs
 
 instance decLt [LT (Prod α β)] [DecidableRel (α:=(Prod α β)) (·<·)] : (n m : Map α β) → Decidable (n < m)
   | .mk nkvs, .mk mkvs => List.hasDecidableLt nkvs mkvs
 
+-- enables ∈ notation for map keys
 instance : Membership α (Map α β) where
   mem a m := List.Mem a (m.kvs.map Prod.fst)
-
-theorem in_list_in_map {α : Type u} (k : α) (v : β) (m : Map α β) :
-  (k, v) ∈ m.kvs → k ∈ m
-:= by
-  intro h₀
-  have h₁ : k ∈ (List.map Prod.fst m.kvs) := by simp ; exists (k, v)
-  apply h₁
-
-theorem contains_iff_some_find? {α β} [BEq α] {m : Map α β} {k : α} :
-  m.contains k ↔ ∃ v, m.find? k = .some v
-:= by simp [contains, Option.isSome_iff_exists]
-
-theorem not_contains_of_empty {α β} [BEq α] (k : α) :
-  ¬ (Map.empty : Map α β).contains k
-:= by simp [contains, empty, find?, List.find?]
 
 end Map
 
