cedar-lean/Cedar/Data/Set.lean
@@ -17,13 +17,16 @@
 import Cedar.Data.List
 import Std.Data.List.Basic
 import Std.Data.List.Lemmas
+
 /-!
+# Canonical list-based sets
+
 This file defines a simple set data type, backed by a sorted duplicate-free
 list. Functions on sets assume but don't require their inputs to be well-formed
 (sorted and duplicate-free). Separate theorems show that these functions produce
 well-formed outputs when given well-formed inputs.
 
-Use Set.make to construct well-formed sets from lists.
+Use `Set.make` to construct well-formed sets from lists.
 -/
 
 namespace Cedar.Data
@@ -34,17 +37,15 @@ deriving Repr, DecidableEq, Inhabited, Lean.ToJson
 
 namespace Set
 
-def elts {α : Type u} : (Set α) -> (List α)
-| .mk elts => elts
-
-open Except
+abbrev elts {α : Type u} (s : Set α) := s.1
 
 ----- Definitions -----
 
--- Creates an ordered/duplicate free list froma  set provided the underlying set is well formed.
+/-- Creates an ordered/duplicate free list from a set provided the underlying
+  set is well formed. -/
 def toList {α : Type u} (s : Set α) : List α := s.elts
 
-/- Creates a well-formed set from the given list. -/
+/-- Creates a well-formed set from the given list. -/
 def make [LT α] [DecidableLT α] (elts : List α) : Set α :=
   Set.mk (elts.canonicalize (·))
 
@@ -56,20 +57,20 @@ def isEmpty {α} [DecidableEq α] (s : Set α) : Bool :=
   s == empty
 
 /-- elt ∈ s -/
-def contains {α} [BEq α] (s : Set α) (elt : α) : Bool :=
+def contains {α} [DecidableEq α] (s : Set α) (elt : α) : Bool :=
   s.elts.elem elt                    -- can use binary search instead
 
 /-- s₁ ⊆ s₂ -/
-def subset {α} [BEq α] (s₁ s₂ : Set α) : Bool :=
+def subset {α} [DecidableEq α] (s₁ s₂ : Set α) : Bool :=
   s₁.elts.all s₂.contains
 
 /-- s₁ ∩ s₂ ≠ ∅ -/
-def intersects {α} [BEq α] (s₁ s₂ : Set α) : Bool :=
+def intersects {α} [DecidableEq α] (s₁ s₂ : Set α) : Bool :=
   s₁.elts.any s₂.contains
 
 /-- s₁ ∩ s₂ -/
-def intersect {α} [BEq α] (s₁ s₂ : Set α) : Set α :=
-  Set.mk (s₁.elts.filter s₂.contains) -- well-formed by construction
+def intersect {α} [DecidableEq α] (s₁ s₂ : Set α) : Set α :=
+  Set.mk (s₁.elts.inter s₂.elts)      -- well-formed by construction
 
 /-- s₁ ∪ s₂ -/
 def union {α} [LT α] [DecidableLT α] (s₁ s₂ : Set α) : Set α :=
@@ -86,8 +87,8 @@ def map {α β} [LT β] [DecidableLT β] (f : α → β) (s : Set α) : Set β :
 /-- Maps `f` to `s` and returns the result of `err` if any error is encountered. -/
 def mapOrErr {α β ε} [DecidableEq β] [LT β] [DecidableRel (α := β) (· < ·)] (f : α → Except ε β) (s : Set α) (err : ε) : Except ε (Set β) :=
   match s.elts.mapM f with
-  | .ok elts => ok (make elts)    -- enforce well-formedness
-  | .error _ => error err         -- return fixed error to be order-independent
+  | .ok elts => .ok (make elts)    -- enforce well-formedness
+  | .error _ => .error err         -- return fixed error to be order-independent
 
 /-- Returns true if all elements of `s` satisfy `f`. -/
 def all {α} (f : α → Bool) (s : Set α) : Bool :=
@@ -106,158 +107,27 @@ def singleton {α} (a : α) : Set α :=
 def foldl {α β} (f : α → β → α) (init : α) (s : Set β) : α :=
   s.elts.foldl f init
 
------ Props and Theorems -----
+----- Instances -----
 
 instance [LT α] : LT (Set α) where
-lt a b := a.elts < b.elts
+  lt a b := a.elts < b.elts
 
-instance decLt [LT α] [DecidableLT α] : (n m : Set α) -> Decidable (n < m)
+instance decLt [LT α] [DecidableLT α] : (n m : Set α) → Decidable (n < m)
   | .mk nelts, .mk melts => List.hasDecidableLt nelts melts
 
-instance : Membership α (Set α) where -- enables ∈ notation
+-- enables ∈
+instance : Membership α (Set α) where
   mem v s := v ∈ s.elts
 
-theorem contains_prop_bool_equiv [DecidableEq α] {v : α} {s : Set α} :
-  s.contains v = true ↔ v ∈ s
-:= by
-  apply Iff.intro
-  intro h0
-  apply List.mem_of_elem_eq_true
-  assumption
-  intro h0
-  apply List.elem_eq_true_of_mem
-  assumption
+-- enables ⊆
+instance [DecidableEq α] : HasSubset (Set α) where
+  Subset s₁ s₂ := s₁.subset s₂
 
-theorem in_list_in_set {α : Type u} (v : α) (s : Set α) :
-  v ∈ s.elts → v ∈ s
-:= by
-  intro h0
-  apply h0
+-- enables ∩
+instance [DecidableEq α] : Inter (Set α) := ⟨Set.intersect⟩
 
-theorem in_set_in_list {α : Type u} (v : α) (s : Set α) :
-  v ∈ s → v ∈ s.elts
-:= by
-  simp [elts, Membership.mem]
-
-theorem mem_cons_self {α : Type u} (hd : α) (tl : List α) :
-  hd ∈ Set.mk (hd :: tl)
-:= by
-  simp [Membership.mem, elts]
-  apply List.mem_cons_self hd tl
-
-theorem mem_cons_of_mem {α : Type u} (a : α) (hd : α) (tl : List α) :
-  a ∈ Set.mk tl → a ∈ Set.mk (hd :: tl)
-:= by
-  simp [Membership.mem, elts] ; intro h₁
-  apply List.mem_cons_of_mem hd h₁
-
-
-theorem in_set_means_list_non_empty {α : Type u} (v : α) (s : Set α) :
-  v ∈ s.elts → ¬(s.elts = [])
-:= by
-  intros h0 h1
-  rw [List.eq_nil_iff_forall_not_mem] at h1
-  specialize h1 v
-  contradiction
-
-theorem make_non_empty [DecidableEq α] [LT α] [DecidableLT α] (xs : List α) :
-  xs ≠ [] ↔ (Set.make xs).isEmpty = false
-:= by
-  unfold isEmpty; unfold empty; unfold make
-  simp only [beq_eq_false_iff_ne, ne_eq, mk.injEq]
-  apply List.canonicalize_not_nil
-
-theorem make_mk_eqv [LT α] [DecidableLT α] [StrictLT α] {xs ys : List α} :
-  Set.make xs = Set.mk ys → xs ≡ ys
-:= by
-  simp [make] ; intro h₁
-  have h₂ := List.canonicalize_equiv xs
-  subst h₁
-  exact h₂
-
-theorem make_make_eqv [LT α] [DecidableLT α] [StrictLT α] {xs ys : List α} :
-  Set.make xs = Set.make ys ↔ xs ≡ ys
-:= by
-  constructor
-  case mp =>
-    intro h; unfold make at h; simp at h
-    have h₁ := List.canonicalize_equiv xs
-    have h₂ := List.canonicalize_equiv ys
-    unfold id at h₁ h₂
-    rw [← h] at h₂
-    have h₃ := List.Equiv.symm h₂; clear h₂
-    exact List.Equiv.trans (a := xs) (b := List.canonicalize (fun x => x) xs) (c := ys) h₁ h₃
-  case mpr =>
-    intro h; unfold make; simp
-    apply List.if_equiv_strictLT_then_canonical _ _ h
-
-theorem make_mem [LT α] [DecidableLT α] [StrictLT α] (x : α) (xs : List α) :
-  x ∈ xs ↔ x ∈ Set.make xs
-:= by
-  simp [make, Membership.mem, elts]
-  have h₁ := List.canonicalize_equiv xs
-  simp [List.Equiv, List.subset_def] at h₁
-  have ⟨h₁, h₂⟩ := h₁
-  constructor <;> intro h₃
-  case mp => apply h₁ h₃
-  case mpr => apply h₂ h₃
-
-theorem elts_make_equiv [LT α] [DecidableLT α] [StrictLT α] {xs : List α} :
-  Set.elts (Set.make xs) ≡ xs
-:= by
-  simp [List.Equiv, List.subset_def]
-  constructor
-  case left =>
-    intro a h₁
-    rw [make_mem]
-    exact in_list_in_set a (make xs) h₁
-  case right =>
-    intro a h₁
-    apply in_set_in_list
-    rw [← make_mem]
-    exact h₁
-
-theorem in_set_in_list' [LT α] [DecidableLT α] [StrictLT α] (v : α) (xs : List α) :
-  v ∈ (Set.make xs) → v ∈ xs
-:= by
-  rw [make_mem]
-  simp
-
-theorem make_any_iff_any [LT α] [DecidableLT α] [StrictLT α] (f : α → Bool) (xs : List α) :
-  (Set.make xs).any f = xs.any f
-:= by
-  simp [make, any, elts]
-  have h₁ := List.canonicalize_equiv xs
-  simp [List.Equiv, List.subset_def] at h₁
-  have ⟨hl₁, hr₁⟩ := h₁
-  cases h₃ : List.any xs f
-  case false =>
-    by_contra h₄
-    simp only [Bool.not_eq_false, List.any_eq_true] at h₄
-    have ⟨x, h₄, h₅⟩ := h₄
-    specialize hr₁ h₄
-    simp [List.any_of_mem hr₁ h₅] at h₃
-  case true =>
-    simp [List.any_eq_true] at *
-    have ⟨x, h₃, h₄⟩ := h₃
-    exists x ; simp [h₄]
-    apply hl₁ h₃
-
-theorem make_of_make_is_id [LT α] [DecidableLT α] [StrictLT α] (xs : List α) :
-  Set.make (Set.elts (Set.make xs)) = Set.make xs
-:= by
-  simp [make, elts]
-  have h₁ := List.canonicalize_id_idempotent xs
-  unfold id at h₁
-  exact h₁
-
-theorem elts_make_is_id_then_equiv [LT α] [DecidableLT α] [StrictLT α] {xs ys : List α} :
-  Set.elts (Set.make xs) = ys → ys ≡ xs
-:= by
-  intro h
-  rw [← h]; clear h
-  rw [← make_make_eqv]
-  exact make_of_make_is_id xs
+-- enables ∪
+instance [LT α] [DecidableLT α] : Union (Set α) := ⟨Set.union⟩
 
 end Set
 
