cedar-lean/Cedar/Thm/Data/List.lean
@@ -1,0 +1,860 @@
+/-
+ Copyright 2022-2023 Amazon.com, Inc. or its affiliates. All Rights Reserved.
+
+ Licensed under the Apache License, Version 2.0 (the "License");
+ you may not use this file except in compliance with the License.
+ You may obtain a copy of the License at
+
+      https://www.apache.org/licenses/LICENSE-2.0
+
+ Unless required by applicable law or agreed to in writing, software
+ distributed under the License is distributed on an "AS IS" BASIS,
+ WITHOUT WARRANTIES OR CONDITIONS OF ANY KIND, either express or implied.
+ See the License for the specific language governing permissions and
+ limitations under the License.
+-/
+
+import Cedar.Data.List
+import Cedar.Data.LT
+import Cedar.Thm.Data.Control
+
+/-!
+
+# List properties
+
+This file contains useful definitions and lemmas about Lists and the additional
+list operators defined in `Cedar.Data.List`.
+
+-/
+
+namespace List
+
+open Cedar.Data
+
+/-! ### Equiv -/
+
+def Equiv {α} (a b : List α) : Prop :=
+  a ⊆ b ∧ b ⊆ a
+
+infix:50 " ≡ " => Equiv
+
+theorem Equiv.refl {a : List α} :
+  a ≡ a
+:= by unfold List.Equiv; simp
+
+theorem Equiv.symm {a b : List α} :
+  a ≡ b → b ≡ a
+:= by unfold List.Equiv; simp; intro h₁ h₂; simp [h₁, h₂]
+
+theorem Equiv.trans {a b c : List α} :
+  a ≡ b → b ≡ c → a ≡ c
+:= by
+  unfold List.Equiv
+  simp only [and_imp]
+  intro h₁ h₂ h₃ h₄
+  apply And.intro
+  exact List.Subset.trans h₁ h₃
+  exact List.Subset.trans h₄ h₂
+
+theorem cons_equiv_cons (x : α) (xs ys : List α) :
+  xs ≡ ys → x :: xs ≡ x :: ys
+:= by
+  unfold List.Equiv
+  intro h₁
+  have ⟨h₁, h₂⟩ := h₁
+  apply And.intro
+  all_goals {
+    apply List.cons_subset_cons; assumption
+  }
+
+theorem dup_head_equiv (x : α) (xs : List α) :
+  x :: x :: xs ≡ x :: xs
+:= by unfold List.Equiv; simp [List.subset_def]
+
+theorem swap_cons_cons_equiv (x₁ x₂ : α) (xs : List α) :
+  x₁ :: x₂ :: xs ≡ x₂ :: x₁ :: xs
+:= by
+  unfold List.Equiv
+  simp only [subset_def, mem_cons, forall_eq_or_imp, true_or, or_true, true_and]
+  apply And.intro
+  all_goals { intro a h₁; simp [h₁] }
+
+theorem filter_equiv (f : α → Bool) (xs ys : List α) :
+  xs ≡ ys → xs.filter f ≡ ys.filter f
+:= by
+  simp only [Equiv, subset_def, and_imp]
+  intros h₁ h₂
+  apply And.intro <;>
+  intro a h₃ <;>
+  simp only [mem_filter] <;>
+  rw [List.mem_filter] at h₃
+  exact And.intro (h₁ h₃.left) h₃.right
+  exact And.intro (h₂ h₃.left) h₃.right
+
+theorem map_equiv (f : α → β) (xs ys : List α) :
+  xs ≡ ys → xs.map f ≡ ys.map f
+:= by
+  intro h
+  have ⟨a, b⟩ := h
+  apply And.intro <;>
+  simp only [subset_def, mem_map, forall_exists_index, and_imp,
+    forall_apply_eq_imp_iff₂] <;>
+  intro p h <;>
+  exists p <;>
+  rw [List.subset_def] at a b <;>
+  simp
+  exact a h
+  exact b h
+
+theorem filterMap_equiv (f : α → Option β) (xs ys : List α) :
+  xs ≡ ys → xs.filterMap f ≡ ys.filterMap f
+:= by
+  simp only [Equiv, subset_def, mem_filterMap, forall_exists_index, and_imp]
+  intros h₁ h₂
+  apply And.intro <;>
+  intro b a h₃ h₄ <;>
+  exists a <;>
+  simp [h₄]
+  exact h₁ h₃
+  exact h₂ h₃
+
+/-! ### Sorted -/
+
+inductive SortedBy [LT β] (f : α → β) : List α → Prop where
+  | nil : SortedBy f []
+  | cons_nil {x} : SortedBy f (x :: nil)
+  | cons_cons {x y ys} :
+      f x < f y →
+      SortedBy f (y :: ys) →
+      SortedBy f (x :: y :: ys)
+
+abbrev Sorted [LT α] (xs : List α) := SortedBy id xs
+
+theorem tail_sortedBy [LT β] {f : α → β} {x : α} {xs : List α} :
+  SortedBy f (x :: xs) → SortedBy f xs
+:= by
+  intro h₁; cases h₁
+  exact SortedBy.nil
+  assumption
+
+theorem sortedBy_implies_head_lt_tail [LT β] [StrictLT β] {f : α → β} {x : α} {xs : List α} :
+  SortedBy f (x :: xs) → ∀ y, y ∈ xs → f x < f y
+:= by
+  intro h₁ y h₂
+  induction xs generalizing y
+  case nil => contradiction
+  case cons _ _ hd tl ih =>
+    cases h₂
+    case head => cases h₁; assumption
+    case tail h₂ =>
+      apply ih
+      case _ =>
+        cases h₁
+        case cons_cons h₃ h₄ =>
+          cases h₄
+          case _ => exact SortedBy.cons_nil
+          case cons_cons _ _ hd' tl' h₅ h₆ =>
+            apply SortedBy.cons_cons _ h₅
+            apply StrictLT.transitive (f x) (f hd) (f hd') h₃ h₆
+      case _ => assumption
+
+theorem sortedBy_equiv_implies_head_eq [LT β] [StrictLT β] (f : α → β) {x y : α} {xs ys : List α} :
+  SortedBy f (x :: xs) →
+  SortedBy f (y :: ys) →
+  (x :: xs) ≡ (y :: ys) →
+  x = y
+:= by
+  intro h₁ h₂
+  unfold List.Equiv; intro h₃
+  replace ⟨h₃, h₄⟩ := h₃
+  simp at h₃; simp at h₄
+  replace ⟨h₃, _⟩ := h₃
+  replace ⟨h₄, _⟩ := h₄
+  cases h₃ <;> cases h₄ <;> try { assumption }
+  case _ _ h₅ => simp [h₅]
+  case _ h₅ h₆ =>
+    have hc₁ := sortedBy_implies_head_lt_tail h₁ y h₆
+    have hc₂ := sortedBy_implies_head_lt_tail h₂ x h₅
+    have hc₃ := StrictLT.asymmetric (f x) (f y) hc₁
+    contradiction
+
+theorem sortedBy_equiv_implies_tail_subset [LT β] [StrictLT β] (f : α → β) {x : α} {xs ys : List α} :
+  SortedBy f (x :: xs) →
+  SortedBy f (x :: ys) →
+  (x :: xs) ⊆ (x :: ys) →
+  xs ⊆ ys
+:= by
+  intro h₁ h₂ h₃
+  simp at h₃
+  simp [List.subset_def]
+  intro y h₄
+  simp [List.subset_def] at h₃
+  specialize h₃ h₄
+  cases h₃
+  case inr => assumption
+  case inl _ h₅ =>
+    subst h₅
+    have h₆ := sortedBy_implies_head_lt_tail h₁ y h₄
+    have h₇ := StrictLT.irreflexive (f y)
+    contradiction
+
+theorem sortedBy_equiv_implies_tail_equiv [LT β] [StrictLT β] (f : α → β) {x : α} {xs ys : List α} :
+  SortedBy f (x :: xs) →
+  SortedBy f (x :: ys) →
+  (x :: xs) ≡ (x :: ys) →
+  xs ≡ ys
+:= by
+  unfold List.Equiv
+  intro h₁ h₂ h₃
+  replace ⟨h₃, h₄⟩ := h₃
+  apply And.intro
+  exact sortedBy_equiv_implies_tail_subset f h₁ h₂ h₃
+  exact sortedBy_equiv_implies_tail_subset f h₂ h₁ h₄
+
+theorem sortedBy_equiv_implies_eq [LT β] [StrictLT β] (f : α → β) {xs ys : List α} :
+  SortedBy f xs → SortedBy f ys → xs ≡ ys → xs = ys
+:= by
+  intro h₁ h₂ h₃
+  induction xs generalizing ys
+  case nil =>
+    apply Eq.symm
+    rw [←List.subset_nil]
+    unfold List.Equiv at h₃
+    exact h₃.right
+  case cons xhd xtl ih =>
+    cases ys
+    case nil =>
+      unfold List.Equiv at h₃
+      rw [←List.subset_nil]
+      exact h₃.left
+    case cons yhd ytl =>
+      simp
+      have h₅ := sortedBy_equiv_implies_head_eq f h₁ h₂ h₃
+      simp only [h₅, true_and]
+      subst h₅
+      apply ih
+      exact (tail_sortedBy h₁)
+      exact (tail_sortedBy h₂)
+      exact (sortedBy_equiv_implies_tail_equiv f h₁ h₂ h₃)
+
+theorem sortedBy_cons [LT β] [StrictLT β] {f : α → β} {x : α} {ys : List α} :
+  SortedBy f ys →
+  (∀ y, y ∈ ys → f x < f y) →
+  SortedBy f (x :: ys)
+:= by
+  intro h₁ h₂
+  cases ys
+  case nil => exact SortedBy.cons_nil
+  case cons hd tl =>
+    apply SortedBy.cons_cons _ h₁
+    apply h₂
+    simp only [mem_cons, true_or]
+
+theorem filter_sortedBy [LT β] [StrictLT β] [DecidableLT β] {f : α → β} (p : α → Bool) {xs : List α} :
+  SortedBy f xs → SortedBy f (xs.filter p)
+:= by
+  intro h₁
+  induction xs
+  case nil => simp only [filter_nil, SortedBy.nil]
+  case cons hd tl ih =>
+    simp only [filter_cons]
+    specialize ih (tail_sortedBy h₁)
+    split
+    case inl =>
+      apply sortedBy_cons ih
+      intro y h₂
+      apply sortedBy_implies_head_lt_tail h₁
+      rw [List.mem_filter] at h₂
+      exact h₂.left
+    case inr => exact ih
+
+/-! ### Forallᵥ -/
+
+def Forallᵥ {α β γ} (p : β → γ → Prop) (kvs₁ : List (α × β)) (kvs₂ : List (α × γ)) : Prop :=
+  List.Forall₂ (fun kv₁ kv₂ => kv₁.fst = kv₂.fst ∧ p kv₁.snd kv₂.snd) kvs₁ kvs₂
+
+
+/-! ### insertCanonical -/
+
+theorem insertCanonical_singleton [LT β] [DecidableLT β] (f : α → β)  (x : α) :
+  insertCanonical f x [] = [x]
+:= by unfold insertCanonical; rfl
+
+theorem insertCanonical_not_nil [DecidableEq β] [LT β] [DecidableLT β] (f : α → β) (x : α) (xs : List α) :
+  insertCanonical f x xs ≠ []
+:= by
+  unfold insertCanonical
+  cases xs with
+  | nil => simp
+  | cons hd tl =>
+    simp
+    intro h
+    split at h <;> try trivial
+    split at h <;> trivial
+
+theorem insertCanonical_sortedBy [LT β] [StrictLT β] [DecidableLT β] {f : α → β} {xs : List α} (x : α) :
+  SortedBy f xs →
+  SortedBy f (insertCanonical f x xs)
+:= by
+  intro h₁
+  induction xs
+  case nil => simp [insertCanonical, SortedBy.cons_nil]
+  case cons hd tl ih =>
+    simp [insertCanonical]
+    split
+    case inl h₂ =>
+      apply SortedBy.cons_cons h₂ h₁
+    case inr h₂ =>
+      split
+      case inl h₃ =>
+        cases h₁
+        case cons_nil =>
+          apply SortedBy.cons_cons h₃
+          apply SortedBy.cons_nil
+        case cons_cons y ys h₄ h₅ =>
+          specialize ih h₄
+          simp [insertCanonical]
+          split
+          case inl h₆ =>
+            apply SortedBy.cons_cons h₃
+            apply SortedBy.cons_cons h₆ h₄
+          case inr h₆ =>
+            split
+            case inl h₇ =>
+              apply SortedBy.cons_cons h₅
+              simp [insertCanonical, h₆, h₇] at ih
+              exact ih
+            case inr h₇ =>
+              have h₈ := StrictLT.if_not_lt_gt_then_eq (f x) (f y) h₆ h₇
+              apply SortedBy.cons_cons h₃
+              cases h₄
+              case cons_nil =>
+                exact SortedBy.cons_nil
+              case cons_cons z zs h₉ h₁₀ =>
+                apply SortedBy.cons_cons (by simp [h₈, h₁₀]) h₉
+      case inr h₃ =>
+        have h₄ := StrictLT.if_not_lt_gt_then_eq (f x) (f hd) h₂ h₃
+        cases h₁
+        case cons_nil =>
+          exact SortedBy.cons_nil
+        case cons_cons h₅ h₆ =>
+          apply SortedBy.cons_cons (by simp only [h₄, h₆]) h₅
+
+theorem insertCanonical_cases [LT β] [DecidableLT β] (f : α → β) (x y : α) (ys : List α) :
+  (f x < f y ∧ insertCanonical f x (y :: ys) = x :: y :: ys) ∨
+  (¬ f x < f y ∧ f x > f y ∧ insertCanonical f x (y :: ys) = y :: insertCanonical f x ys) ∨
+  (¬ f x < f y ∧ ¬ f x > f y ∧ insertCanonical f x (y :: ys) = x :: ys)
+:= by
+  generalize h₁ : insertCanonical f x ys = xys
+  unfold insertCanonical; simp
+  by_cases (f x < f y)
+  case pos _ _ h₂ => simp [h₂]
+  case neg _ _ h₂ =>
+    simp [h₂]
+    by_cases (f x > f y)
+    case pos _ _ h₃ => simp [h₃, h₁]
+    case neg _ _ h₃ => simp [h₃]
+
+theorem insertCanonical_equiv [LT α] [StrictLT α] [DecidableLT α] (x : α) (xs : List α) :
+  x :: xs ≡ insertCanonical id x xs
+:= by
+  unfold insertCanonical
+  induction xs
+  case nil => simp; exact Equiv.refl
+  case cons _ _ hd tl ih =>
+    simp
+    split
+    case inl => exact Equiv.refl
+    case inr _ _ h₁ =>
+      split
+      case inr _ _ h₂ =>
+        have h₃ := StrictLT.if_not_lt_gt_then_eq x hd h₁ h₂
+        subst h₃
+        exact dup_head_equiv x tl
+      case inl _ _ h₂ =>
+        cases tl
+        case nil =>
+          have h₃ := insertCanonical_singleton id x
+          simp [h₃]
+          apply swap_cons_cons_equiv
+        case cons _ _ _ hd' tl' =>
+          simp at ih
+          have h₃ := insertCanonical_cases id x hd' tl'
+          simp only [id_eq] at h₃
+          cases h₃
+          case inl _ _ _ h₃ =>
+            simp [h₃]
+            unfold List.Equiv
+            simp only [cons_subset, mem_cons, true_or, or_true, true_and]
+            apply And.intro
+            all_goals {
+              simp [List.subset_def]
+              intro a h₄; simp [h₄]
+            }
+          case inr _ _ _ h₃ =>
+            cases h₃
+            case inr _ _ _ h₃ =>
+              replace ⟨h₃, h₄, h₅⟩ := h₃
+              simp [h₅]
+              unfold GT.gt at h₄
+              have h₆ := StrictLT.if_not_lt_gt_then_eq x hd' h₃ h₄
+              subst h₆
+              unfold List.Equiv
+              simp only [cons_subset, mem_cons, true_or, or_true, Subset.refl, and_self, subset_cons]
+            case inl _ _ _ h₃ =>
+              replace ⟨h₃, h₄, h₅⟩ := h₃
+              simp [h₅]
+              simp [h₃, h₄] at ih
+              have h₆ := swap_cons_cons_equiv x hd (hd' :: tl')
+              apply Equiv.trans h₆
+              apply cons_equiv_cons
+              exact ih
+
+theorem insertCanonical_preserves_forallᵥ {α β γ} [LT α] [StrictLT α] [DecidableLT α] {p : β → γ → Prop}
+  {kv₁ : α × β} {kv₂ : α × γ} {kvs₁ : List (α × β)} {kvs₂ : List (α × γ)}
+  (h₁ : kv₁.fst = kv₂.fst ∧ p kv₁.snd kv₂.snd)
+  (h₂ : Forallᵥ p kvs₁ kvs₂) :
+  Forallᵥ p (insertCanonical Prod.fst kv₁ kvs₁) (insertCanonical Prod.fst kv₂ kvs₂)
+:= by
+  simp [Forallᵥ] at *
+  cases h₂
+  case nil =>
+    simp [insertCanonical_singleton]
+    apply Forall₂.cons (by exact h₁) (by simp only [Forall₂.nil])
+  case cons hd₁ hd₂ tl₁ tl₂ h₃ h₄ =>
+    simp [insertCanonical]
+    split <;> split
+    case inl.inl =>
+      apply Forall₂.cons (by exact h₁)
+      apply Forall₂.cons (by exact h₃) (by exact h₄)
+    case inl.inr h₅ h₆ =>
+      simp [h₁, h₃] at h₅
+      have _ := StrictLT.asymmetric kv₂.fst hd₂.fst h₅
+      split <;> contradiction
+    case inr.inl h₅ h₆ =>
+      simp [h₁, h₃] at h₅ h₆
+      split
+      case inl => contradiction
+      case inr =>
+        apply Forall₂.cons (by exact h₃)
+        apply insertCanonical_preserves_forallᵥ h₁ h₄
+    case inr.inr h₅ h₆ =>
+      simp [h₁, h₃] at h₅ h₆
+      split
+      case inl => contradiction
+      case inr => apply Forall₂.cons (by exact h₁) (by exact h₄)
+
+theorem insertCanonical_map_fst {α β γ} [LT α] [StrictLT α] [DecidableLT α] (xs : List (α × β)) (f : β → γ) (x : α × β) :
+  insertCanonical Prod.fst (Prod.map id f x) (map (Prod.map id f) xs) =
+  map (Prod.map id f) (insertCanonical Prod.fst x xs)
+:= by
+  induction xs generalizing x
+  case nil => simp [insertCanonical, canonicalize, Prod.map]
+  case cons ih =>
+    simp [insertCanonical, Prod.map]
+    split
+    case inl => simp [Prod.map]
+    case inr =>
+      split
+      case inl => specialize ih x ; simp [Prod.map] at ih ; simp [ih, Prod.map]
+      case inr => simp [Prod.map]
+
+theorem insertCanonical_map_fst_canonicalize {α β γ} [LT α] [StrictLT α] [DecidableLT α] (xs : List (α × β)) (f : β → γ) (x : α × β) :
+  insertCanonical Prod.fst (Prod.map id f x) (canonicalize Prod.fst (map (Prod.map id f) xs)) =
+  map (Prod.map id f) (insertCanonical Prod.fst x (canonicalize Prod.fst xs))
+:= by
+  induction xs generalizing x
+  case nil =>
+    simp [insertCanonical, canonicalize, Prod.map]
+  case cons hd tl ih =>
+    simp [canonicalize, ih hd]
+    apply insertCanonical_map_fst (insertCanonical Prod.fst hd (canonicalize Prod.fst tl))
+
+/-! ## canonicalize -/
+
+theorem canonicalize_nil [LT β] [DecidableLT β] (f : α → β) :
+  canonicalize f [] = []
+:= by unfold canonicalize; rfl
+
+theorem canonicalize_not_nil [DecidableEq β] [LT β] [DecidableLT β] (f : α → β) (xs : List α) :
+  xs ≠ [] ↔ (canonicalize f xs) ≠ []
+:= by
+  apply Iff.intro
+  case _ =>
+    intro h₀
+    cases xs with
+    | nil => contradiction
+    | cons hd tl =>
+      unfold canonicalize
+      apply insertCanonical_not_nil
+  case _ =>
+    unfold canonicalize
+    intro h₀
+    cases xs <;> simp at h₀; simp
+
+theorem canonicalize_sortedBy [LT β] [StrictLT β] [DecidableLT β] (f : α → β) (xs : List α) :
+  SortedBy f (canonicalize f xs)
+:= by
+  induction xs
+  case nil => simp [canonicalize_nil, SortedBy.nil]
+  case cons _ _ hd tl ih =>
+    unfold canonicalize
+    apply insertCanonical_sortedBy
+    exact ih
+
+theorem sortedBy_implies_canonicalize_eq [LT β] [StrictLT β] [DecidableLT β] {f : α → β} {xs : List α} :
+  SortedBy f xs → (canonicalize f xs) = xs
+:= by
+  intro h₁
+  induction xs
+  case nil => simp [canonicalize]
+  case cons hd tl ih =>
+    simp [canonicalize]
+    cases h₁
+    case cons_nil => simp [canonicalize, insertCanonical]
+    case cons_cons h₁ h₂ =>
+      specialize ih h₁
+      simp [ih, insertCanonical, h₂]
+
+/-
+Note that `canonicalize_equiv` does not hold for all functions `f`.
+To see why, consider xs = [(1, false), (1, true)], f = Prod.fst.
+Then `canonicalize f xs = [(1, false)] !≡ xs`.
+-/
+theorem canonicalize_equiv [LT α] [StrictLT α] [DecidableLT α] (xs : List α) :
+  xs ≡ canonicalize id xs
+:= by
+  induction xs
+  case nil => simp [canonicalize_nil, Equiv.refl]
+  case cons _ _ hd tl ih =>
+    unfold canonicalize
+    generalize h₁ : canonicalize id tl = ys
+    simp [h₁] at ih
+    have h₂ := insertCanonical_equiv hd ys
+    apply Equiv.trans _ h₂
+    apply cons_equiv_cons
+    exact ih
+
+theorem equiv_implies_canonical_eq [LT α] [StrictLT α] [DecidableLT α] (xs ys : List α) :
+  xs ≡ ys → (canonicalize id xs) = (canonicalize id ys)
+:= by
+  intro h₁
+  apply sortedBy_equiv_implies_eq id
+  exact (canonicalize_sortedBy id xs)
+  exact (canonicalize_sortedBy id ys)
+  have h₂ := Equiv.symm (canonicalize_equiv xs)
+  have h₃ := Equiv.symm (canonicalize_equiv ys)
+  apply Equiv.trans h₂
+  apply Equiv.symm
+  apply Equiv.trans h₃
+  apply Equiv.symm
+  exact h₁
+
+theorem canonicalize_idempotent {α β} [LT β] [StrictLT β] [DecidableLT β] (f : α → β) (xs : List α) :
+  canonicalize f (canonicalize f xs) = canonicalize f xs
+:= sortedBy_implies_canonicalize_eq (canonicalize_sortedBy f xs)
+
+/-
+Note that a more general version of `canonicalize_id_filter` does not hold.
+In particular, we can't replace `id` with an arbitrary function `f`.
+To see why, consider xs = [(1, false), (1, true)], f = Prod.fst, p = Prod.snd.
+Then `(canonicalize f xs).filter p = []` but `(xs.filter p).canonicalize f = [(1, true)]`.
+
+#eval (canonicalize Prod.fst [(1, false), (1, true)]).filter Prod.snd
+#eval ([(1, false), (1, true)].filter Prod.snd).canonicalize Prod.fst
+-/
+theorem canonicalize_id_filter {α} [LT α] [StrictLT α] [DecidableLT α] (p : α → Bool) (xs : List α) :
+  (canonicalize id xs).filter p = (xs.filter p).canonicalize id
+:= by
+  have h₁ : (canonicalize id xs).filter p ≡ xs.filter p := by
+    apply filter_equiv
+    apply Equiv.symm
+    apply canonicalize_equiv
+  have h₂ := canonicalize_equiv (filter p xs)
+  exact sortedBy_equiv_implies_eq id
+    (filter_sortedBy p (canonicalize_sortedBy id xs))
+    (canonicalize_sortedBy id (filter p xs))
+    (Equiv.trans h₁ h₂)
+
+theorem canonicalize_preserves_forallᵥ {α β γ} [LT α] [StrictLT α] [DecidableLT α] (p : β → γ → Prop) (kvs₁ : List (α × β)) (kvs₂ : List (α × γ)) :
+  List.Forallᵥ p kvs₁ kvs₂ →
+  List.Forallᵥ p (List.canonicalize Prod.fst kvs₁) (List.canonicalize Prod.fst kvs₂)
+:= by
+  simp [Forallᵥ]
+  intro h₁
+  cases h₁
+  case nil => simp [canonicalize_nil]
+  case cons hd₁ hd₂ tl₁ tl₂ h₂ h₃ =>
+    simp [canonicalize]
+    have h₄ := canonicalize_preserves_forallᵥ p tl₁ tl₂ h₃
+    apply insertCanonical_preserves_forallᵥ h₂ h₄
+
+theorem canonicalize_of_map_fst {α β γ} [LT α] [StrictLT α] [DecidableLT α] (xs : List (α × β)) (f : β → γ) :
+  List.canonicalize Prod.fst (List.map (Prod.map id f) xs) =
+  List.map (Prod.map id f) (List.canonicalize Prod.fst xs)
+:= by
+  cases xs
+  case nil => simp [canonicalize]
+  case cons hd tl =>
+    simp [canonicalize]
+    exact insertCanonical_map_fst_canonicalize tl f hd
+
+/-! ### any -/
+
+theorem any_of_mem {f : α → Bool} {x : α} {xs : List α}
+  (h₁ : x ∈ xs)
+  (h₂ : f x) :
+  any xs f = true
+:= by
+  cases xs <;> simp at h₁
+  case cons hd tl =>
+    simp [List.any_cons]
+    rcases h₁ with h₁ | h₁
+    subst h₁ ; simp [h₂]
+    apply Or.inr ; exists x
+
+/-! ### mapM and mapM₁ -/
+
+theorem mapM_pmap_subtype [Monad m] [LawfulMonad m]
+  {p : α → Prop}
+  (f : α → m β)
+  (as : List α)
+  (h : ∀ a, a ∈ as → p a)
+  : List.mapM (fun x : { a : α // p a } => f x.val) (List.pmap Subtype.mk as h)
+    =
+    List.mapM f as
+:= by
+  rw [←List.mapM'_eq_mapM]
+  induction as <;> simp [*]
+
+theorem mapM₁_eq_mapM [Monad m] [LawfulMonad m]
+  (f : α → m β)
+  (as : List α) :
+  List.mapM₁ as (fun x : { x // x ∈ as } => f x.val) =
+  List.mapM f as
+:= by
+  simp [mapM₁, attach, mapM_pmap_subtype]
+
+theorem mapM_implies_nil {f : α → Except β γ} {as : List α}
+  (h₁ : List.mapM f as = Except.ok []) :
+  as = []
+:= by
+  rw [←List.mapM'_eq_mapM] at h₁
+  cases as
+  case nil => rfl
+  case cons hd tl =>
+    simp [List.mapM'] at h₁
+    cases h₂ : f hd <;> simp [h₂] at h₁
+    cases h₃ : List.mapM' f tl <;>
+    simp [h₃, pure, Except.pure] at h₁
+
+theorem mapM_head_tail {α β γ} {f : α → Except β γ} {x : α} {xs : List α} {y : γ} {ys : List γ} :
+  (List.mapM f (x :: xs)) = Except.ok (y :: ys) →
+  (List.mapM f xs) = Except.ok ys
+:= by
+  simp [←List.mapM'_eq_mapM]
+  cases h₁ : f x <;>
+  simp [h₁]
+  cases h₂ : mapM' f xs <;>
+  simp [h₂, pure, Except.pure]
+
+/-! ### foldlM -/
+
+theorem foldlM_of_assoc_some (f : α → α → Option α) (x₀ x₁ x₂ x₃ : α) (xs : List α)
+  (h₁ : ∀ x₁ x₂ x₃,
+    (do let x₄ ← f x₁ x₂ ; f x₄ x₃) =
+    (do let x₄ ← f x₂ x₃ ; f x₁ x₄))
+  (h₂ : f x₀ x₁ = some x₂)
+  (h₃ : List.foldlM f x₂ xs = some x₃):
+  (do let y ← List.foldlM f x₁ xs ; f x₀ y) = some x₃
+:= by
+  cases xs
+  case nil =>
+    simp [List.foldlM, pure] at *
+    subst h₃; exact h₂
+  case cons hd tl =>
+    simp [List.foldlM] at *
+    cases h₄ : f x₂ hd <;> simp [h₄] at h₃
+    rename_i x₄
+    have h₅ := h₁ x₀ x₁ hd
+    simp [h₂, h₄] at h₅
+    cases h₆ : f x₁ hd <;> simp [h₆] at h₅
+    rename_i x₅
+    have h₇ := List.foldlM_of_assoc_some f x₂ hd x₄ x₃ tl h₁ h₄ h₃
+    cases h₈ : List.foldlM f hd tl <;> simp [h₈] at h₇
+    rename_i x₆
+    rw [eq_comm] at h₅
+    cases h₉ : List.foldlM f x₅ tl <;> simp [h₉]
+    case none =>
+      have h₁₀ := List.foldlM_of_assoc_some f x₀ x₅ x₄ x₃ tl h₁ h₅ h₃
+      simp [h₉] at h₁₀
+    case some x₇ =>
+      have h₁₀ := List.foldlM_of_assoc_some f x₁ hd x₅ x₇ tl h₁ h₆ h₉
+      simp [h₈] at h₁₀
+      specialize h₁ x₀ x₁ x₆
+      simp [h₂, h₁₀] at h₁
+      simp [←h₁, h₇]
+
+theorem foldlM_of_assoc_none' (f : α → α → Option α) (x₀ x₁ x₂ : α) (xs : List α)
+  (h₁ : ∀ x₁ x₂ x₃,
+    (do let x₄ ← f x₁ x₂ ; f x₄ x₃) =
+    (do let x₄ ← f x₂ x₃ ; f x₁ x₄))
+  (h₂ : f x₀ x₁ = none)
+  (h₃ : List.foldlM f x₁ xs = some x₂):
+  f x₀ x₂ = none
+:= by
+  cases xs
+  case nil =>
+    simp [pure] at h₃ ; subst h₃; exact h₂
+  case cons hd tl =>
+    simp [List.foldlM] at h₃
+    cases h₄ : f x₁ hd <;> simp [h₄] at h₃
+    rename_i x₃
+    have h₅ := List.foldlM_of_assoc_some f x₁ hd x₃ x₂ tl h₁ h₄ h₃
+    cases h₆ : List.foldlM f hd tl <;> simp [h₆] at h₅
+    rename_i x₄
+    specialize h₁ x₀ x₁ x₄
+    simp [h₂, h₅] at h₁
+    simp [h₁]
+
+theorem foldlM_of_assoc_none (f : α → α → Option α) (x₀ x₁ x₂ : α) (xs : List α)
+  (h₁ : ∀ x₁ x₂ x₃,
+    (do let x₄ ← f x₁ x₂ ; f x₄ x₃) =
+    (do let x₄ ← f x₂ x₃ ; f x₁ x₄))
+  (h₂ : f x₀ x₁ = some x₂)
+  (h₃ : List.foldlM f x₂ xs = none):
+  (do let y ← List.foldlM f x₁ xs ; f x₀ y) = none
+:= by
+  cases xs
+  case nil =>
+    simp [List.foldlM] at h₃
+  case cons hd tl =>
+    simp [List.foldlM]
+    cases h₄ : f x₁ hd <;> simp [h₄]
+    rename_i x₃
+    cases h₅ : List.foldlM f x₃ tl <;> simp [h₅]
+    rename_i x₄
+    have h₆ := List.foldlM_of_assoc_some f x₁ hd x₃ x₄ tl h₁ h₄ h₅
+    cases h₇ : List.foldlM f hd tl <;> simp [h₇] at h₆
+    rename_i x₅
+    simp [List.foldlM] at h₃
+    cases h₈ : f x₂ hd <;> simp [h₈] at h₃
+    case none =>
+      have h₉ := List.foldlM_of_assoc_none' f x₂ hd x₅ tl h₁ h₈ h₇
+      have h₁₀ := h₁ x₀ x₁ x₅
+      simp [h₂, h₆] at h₁₀
+      simp [←h₁₀, h₉]
+    case some x₆ =>
+      have h₉ := List.foldlM_of_assoc_none f x₂ hd x₆ tl h₁ h₈ h₃
+      simp [h₇] at h₉
+      have h₁₀ := h₁ x₀ x₁ x₅
+      simp [h₂, h₆] at h₁₀
+      simp [←h₁₀, h₉]
+
+theorem foldlM_of_assoc (f : α → α → Option α) (x₀ x₁ : α) (xs : List α)
+  (h₁ : ∀ x₁ x₂ x₃,
+    (do let x₄ ← f x₁ x₂ ; f x₄ x₃) =
+    (do let x₄ ← f x₂ x₃ ; f x₁ x₄) ) :
+  List.foldlM f x₀ (x₁ :: xs) =
+  (do let y ← List.foldlM f x₁ xs ; f x₀ y)
+:= by
+  simp [List.foldlM]
+  cases h₂ : f x₀ x₁ <;> simp [h₂]
+  case none =>
+    induction xs generalizing x₁
+    case nil => simp [h₂]
+    case cons hd tl ih =>
+      simp [List.foldlM]
+      cases h₃ : f x₁ hd <;> simp [h₃]
+      rename_i x₂
+      specialize h₁ x₀ x₁ hd
+      simp [h₂, h₃] at h₁
+      specialize ih x₂
+      apply ih
+      rw [eq_comm] at h₁ ; exact h₁
+  case some x₂ =>
+    rw [eq_comm]
+    cases h₃ : List.foldlM f x₂ xs
+    case none =>
+      exact List.foldlM_of_assoc_none f x₀ x₁ x₂ xs h₁ h₂ h₃
+    case some x₃ =>
+      exact List.foldlM_of_assoc_some f x₀ x₁ x₂ x₃ xs h₁ h₂ h₃
+
+/-! ### find? -/
+
+theorem find?_pair_map {α β γ} [BEq α] (f : β → γ) (xs : List (α × β)) (k : α)  :
+  Option.map (λ x => (x.fst, f x.snd)) (List.find? (λ x => x.fst == k) xs)  =
+  List.find? (λ x => x.fst == k) (List.map (λ x => (x.fst, f x.snd)) xs)
+:= by
+  induction xs
+  case nil =>
+    simp only [find?_nil, Option.map_none', map_nil]
+  case cons hd tl ih =>
+    cases h₁ : hd.fst == k <;> simp only [map_cons]
+    case false =>
+      rw [Bool.eq_false_iff, ne_eq] at h₁
+      have h₂ := @List.find?_cons_of_neg _
+        (λ (x : α × β) => x.fst == k) hd tl h₁
+      have h₃ := @List.find?_cons_of_neg _
+        (λ (x : α × γ) => x.fst == k) (hd.fst, f hd.snd)
+        (map (fun x => (x.fst, f x.snd)) tl)
+      simp [h₁] at h₃
+      simp [h₂, h₃]
+      exact ih
+    case true =>
+      have h₂ := @List.find?_cons_of_pos _
+        (λ (x : α × β) => x.fst == k) hd tl h₁
+      have h₃ := @List.find?_cons_of_pos _
+        (λ (x : α × γ) => x.fst == k) (hd.fst, f hd.snd)
+        (map (fun x => (x.fst, f x.snd)) tl)
+      simp [h₁] at h₃
+      simp [h₂, h₃]
+
+theorem find?_fst_map_implies_find? {α β γ} [BEq α] {f : β → γ} {xs : List (α × β)} {k : α} {fx : α × γ}:
+  List.find? (fun x => x.fst == k) (List.map (Prod.map id f) xs) = .some fx  →
+  ∃ x, xs.find? (fun x => x.fst == k) = .some x ∧ fx = Prod.map id f x
+:= by
+  intro h
+  induction xs
+  case nil =>
+    simp only [map_nil, find?_nil] at h
+  case cons hd tl ih =>
+    simp only [map_cons, find?_cons] at h
+    split at h
+    case h_1 heq =>
+      exists hd
+      simp only [Option.some.injEq] at h
+      simp only [h, and_true]
+      simp only [Prod.map, id_eq] at heq
+      simp only [find?_cons, heq]
+    case h_2 heq =>
+      replace ⟨x, ih⟩ := ih h
+      exists x
+      simp only [Prod.map, id_eq] at heq
+      simp only [find?_cons, heq, ih, and_self]
+
+/-! ### map -/
+
+/-
+These are copied from Mathlib. We can delete them if they get added to Std.
+-/
+
+theorem map_pmap_subtype
+  {p : α → Prop}
+  (f : α → β)
+  (as : List α)
+  (h : ∀ a, a ∈ as → p a)
+  : List.map (fun x : { a : α // p a } => f x.val) (List.pmap Subtype.mk as h)
+    =
+    List.map f as
+:= by
+  induction as <;> simp [*]
+
+theorem map_congr {f g : α → β} : ∀ {l : List α},
+  (∀ x ∈ l, f x = g x) → map f l = map g l
+  | [], _ => rfl
+  | a :: l, h => by
+    let ⟨h₁, h₂⟩ := forall_mem_cons.1 h
+    rw [map, map, h₁, map_congr h₂]
+
+end List
