cedar-lean/Cedar/Thm/Data/Set.lean
@@ -1,0 +1,207 @@
+/-
+ Copyright 2022-2023 Amazon.com, Inc. or its affiliates. All Rights Reserved.
+
+ Licensed under the Apache License, Version 2.0 (the "License");
+ you may not use this file except in compliance with the License.
+ You may obtain a copy of the License at
+
+      https://www.apache.org/licenses/LICENSE-2.0
+
+ Unless required by applicable law or agreed to in writing, software
+ distributed under the License is distributed on an "AS IS" BASIS,
+ WITHOUT WARRANTIES OR CONDITIONS OF ANY KIND, either express or implied.
+ See the License for the specific language governing permissions and
+ limitations under the License.
+-/
+
+import Cedar.Data.Set
+import Cedar.Thm.Data.Control
+import Cedar.Thm.Data.List
+
+/-!
+# Set properties
+
+This file proves useful properties of canonical list-based sets defined in
+`Cedar.Data.Set`.
+-/
+
+namespace Cedar.Data.Set
+
+/-! ### Well-formed sets -/
+
+def WellFormed {α} [LT α] [DecidableLT α] (s : Set α) :=
+  s = Set.make s.toList
+
+/-! ### contains and mem -/
+
+theorem contains_prop_bool_equiv [DecidableEq α] {v : α} {s : Set α} :
+  s.contains v = true ↔ v ∈ s
+:= by
+  apply Iff.intro
+  intro h0
+  apply List.mem_of_elem_eq_true
+  assumption
+  intro h0
+  apply List.elem_eq_true_of_mem
+  assumption
+
+theorem in_list_in_set {α : Type u} (v : α) (s : Set α) :
+  v ∈ s.elts → v ∈ s
+:= by
+  intro h0
+  apply h0
+
+theorem in_set_in_list {α : Type u} (v : α) (s : Set α) :
+  v ∈ s → v ∈ s.elts
+:= by
+  simp [Membership.mem]
+
+theorem mem_cons_self {α : Type u} (hd : α) (tl : List α) :
+  hd ∈ Set.mk (hd :: tl)
+:= by
+  simp only [Membership.mem]
+  apply List.mem_cons_self hd tl
+
+theorem mem_cons_of_mem {α : Type u} (a : α) (hd : α) (tl : List α) :
+  a ∈ Set.mk tl → a ∈ Set.mk (hd :: tl)
+:= by
+  simp only [Membership.mem] ; intro h₁
+  apply List.mem_cons_of_mem hd h₁
+
+theorem in_set_means_list_non_empty {α : Type u} (v : α) (s : Set α) :
+  v ∈ s.elts → ¬(s.elts = [])
+:= by
+  intros h0 h1
+  rw [List.eq_nil_iff_forall_not_mem] at h1
+  specialize h1 v
+  contradiction
+
+/-! ### isEmpty -/
+
+theorem make_non_empty [DecidableEq α] [LT α] [DecidableLT α] (xs : List α) :
+  xs ≠ [] ↔ (Set.make xs).isEmpty = false
+:= by
+  unfold isEmpty; unfold empty; unfold make
+  simp only [beq_eq_false_iff_ne, ne_eq, mk.injEq]
+  apply List.canonicalize_not_nil
+
+/-! ### make -/
+
+theorem make_mem [LT α] [DecidableLT α] [StrictLT α] (x : α) (xs : List α) :
+  x ∈ xs ↔ x ∈ Set.make xs
+:= by
+  simp only [Membership.mem, make]
+  have h₁ := List.canonicalize_equiv xs
+  simp [List.Equiv, List.subset_def] at h₁
+  have ⟨h₁, h₂⟩ := h₁
+  constructor <;> intro h₃
+  case mp => apply h₁ h₃
+  case mpr => apply h₂ h₃
+
+theorem make_mk_eqv [LT α] [DecidableLT α] [StrictLT α] {xs ys : List α} :
+  Set.make xs = Set.mk ys → xs ≡ ys
+:= by
+  simp [make] ; intro h₁
+  have h₂ := List.canonicalize_equiv xs
+  subst h₁
+  exact h₂
+
+theorem make_make_eqv [LT α] [DecidableLT α] [StrictLT α] {xs ys : List α} :
+  Set.make xs = Set.make ys ↔ xs ≡ ys
+:= by
+  constructor
+  case mp =>
+    intro h; unfold make at h; simp at h
+    have h₁ := List.canonicalize_equiv xs
+    have h₂ := List.canonicalize_equiv ys
+    unfold id at h₁ h₂
+    rw [← h] at h₂
+    have h₃ := List.Equiv.symm h₂; clear h₂
+    exact List.Equiv.trans (a := xs) (b := List.canonicalize (fun x => x) xs) (c := ys) h₁ h₃
+  case mpr =>
+    intro h; unfold make; simp
+    apply List.equiv_implies_canonical_eq _ _ h
+
+theorem elts_make_equiv [LT α] [DecidableLT α] [StrictLT α] {xs : List α} :
+  Set.elts (Set.make xs) ≡ xs
+:= by
+  simp [List.Equiv, List.subset_def]
+  constructor
+  case left =>
+    intro a h₁
+    rw [make_mem]
+    exact in_list_in_set a (make xs) h₁
+  case right =>
+    intro a h₁
+    apply in_set_in_list
+    rw [← make_mem]
+    exact h₁
+
+theorem in_set_in_list' [LT α] [DecidableLT α] [StrictLT α] (v : α) (xs : List α) :
+  v ∈ (Set.make xs) → v ∈ xs
+:= by
+  rw [make_mem]
+  simp
+
+theorem make_any_iff_any [LT α] [DecidableLT α] [StrictLT α] (f : α → Bool) (xs : List α) :
+  (Set.make xs).any f = xs.any f
+:= by
+  simp [make, any]
+  have h₁ := List.canonicalize_equiv xs
+  simp [List.Equiv, List.subset_def] at h₁
+  have ⟨hl₁, hr₁⟩ := h₁
+  cases h₃ : List.any xs f
+  case false =>
+    by_contra h₄
+    simp only [Bool.not_eq_false, List.any_eq_true] at h₄
+    have ⟨x, h₄, h₅⟩ := h₄
+    specialize hr₁ h₄
+    simp [List.any_of_mem hr₁ h₅] at h₃
+  case true =>
+    simp [List.any_eq_true] at *
+    have ⟨x, h₃, h₄⟩ := h₃
+    exists x ; simp [h₄]
+    apply hl₁ h₃
+
+theorem make_of_make_is_id [LT α] [DecidableLT α] [StrictLT α] (xs : List α) :
+  Set.make (Set.elts (Set.make xs)) = Set.make xs
+:= by
+  simp only [make, mk.injEq]
+  have h₁ := List.canonicalize_idempotent id xs
+  unfold id at h₁
+  exact h₁
+
+theorem elts_make_is_id_then_equiv [LT α] [DecidableLT α] [StrictLT α] {xs ys : List α} :
+  Set.elts (Set.make xs) = ys → ys ≡ xs
+:= by
+  intro h
+  rw [← h]; clear h
+  rw [← make_make_eqv]
+  exact make_of_make_is_id xs
+
+/-! ### inter -/
+
+theorem mem_inter_iff {α} [DecidableEq α] {x : α} {s₁ s₂ : Set α} :
+  x ∈ s₁ ∩ s₂ ↔ x ∈ s₁ ∧ x ∈ s₂
+:= by
+  simp only [Membership.mem, intersect]
+  rename_i iDecEq
+  have h := @List.mem_inter_iff α iDecEq x s₁.1 s₂.1
+  simp only [Membership.mem, Inter.inter] at h
+  exact h
+
+theorem inter_wf {α} [LT α] [StrictLT α] [DecidableLT α] [DecidableEq α] {s₁ s₂ : Set α}
+ (h₁ : WellFormed s₁) :
+ WellFormed (s₁ ∩ s₂)
+:= by
+  simp only [WellFormed] at *
+  simp only [Inter.inter, intersect]
+  simp only [make, toList, elts, mk.injEq] at *
+  simp only [List.inter]
+  rename_i iLT iSLT iDecLT iDecEq
+  have h₃ := @List.canonicalize_id_filter α iLT iSLT iDecLT (fun x => decide (x ∈ s₂.1)) s₁.1
+  rw (config := {occs := .pos [1]}) [h₁]
+  simp only
+  apply h₃
+
+end Cedar.Data.Set
